theories/Set.ec
@@ -22,9 +22,17 @@ op card     : 'a t -> int.
 
 axiom card_pos : forall (X:'a t), 0 <= card X. 
 
+pred [==] (X1:'a t, X2:'a t) = 
+  forall (x:'a), mem x X1 <=> mem x X2.
+
+axiom extentionnality : 
+  forall (X1:'a t, X2:'a t),
+     X1 = X2 <=> X1 == X2.
+
 (* Specification of is_empty *)
 axiom is_empty_mem : forall (X:'a t), 
    is_empty X <=> forall (x:'a), !mem x X.
+
 axiom is_empty_card : forall (X:'a t),
    is_empty X <=> card X = 0.
 
@@ -34,20 +42,24 @@ axiom is_empty_empty : is_empty<:'a> empty<:'a>.
 (* FIXME lemma *)
 axiom empty_mem  : forall (x:'a), !mem x empty.
 
-lemma empty_card : card<:'a>(empty) = 0.
+axiom empty_card : card<:'a>(empty) = 0.
 
 (* Specification of add *)
 
 axiom add_mem : forall (x:'a, y:'a, X:'a t), 
    mem x (add y X) <=> mem x X || x = y.
 
+axiom add_card : forall (x:'a, X:'a t), 
+   !mem x X => card (add x X) = card X + 1.
+
 (* Need to put extentionality, to get it as a lemma *)
 axiom mem_add : forall (x:'a, X:'a t),
    mem x X => X = add x X.
 
-axiom add_card : forall (x:'a, X:'a t), 
-   !mem x X => card (add x X) = 1 + card X. 
+axiom singleton_card : forall (x:'a),
+   card (singleton x) = 1.
 
+(* filter *)
 op filter : ('a Pred, 'a t) -> 'a t.
 
 axiom filter_mem : forall (P:'a Pred, X:'a t, x:'a),
@@ -56,4 +68,13 @@ axiom filter_mem : forall (P:'a Pred, X:'a t, x:'a),
 axiom filter_card : forall (P:'a Pred, X : 'a t), 
    card (filter P X) = card X - card(filter (Pnot P) X). 
 
+axiom filter_Peq_in : forall (x:'a, X:'a t),
+   mem x X =>
+   filter (Peq x) X = singleton x.
+
+axiom filter_Peq_card_in : forall (x:'a, X:'a t),
+   mem x X =>
+   card (filter (Peq x) X) = 1.
+     
+  
 
